crates/algorithms/sha3/proofs/fstar/extraction/Libcrux_sha3.Neon.fst
@@ -19,17 +19,23 @@ let sha224 (digest data: t_Slice u8)
             bool) /\
           (digest_future <: t_Slice u8) ==
           (Hacspec_sha3.Sponge.keccak (Core_models.Slice.impl__len #u8 digest)
-              (mk_usize 144) (mk_u8 6) data
+              (mk_usize 144)
+              (mk_u8 6)
+              data
             <:
             t_Slice u8)) =
   let dummy:t_Array u8 (mk_usize 28) = Rust_primitives.Hax.repeat (mk_u8 0) (mk_usize 28) in
   let _:Prims.unit =
-    let inputs : t_Array (t_Slice u8) (mk_usize 2) =
-      let l : list (t_Slice u8) = [ data; data ] in
+    let inputs:t_Array (t_Slice u8) (mk_usize 2) =
+      let l:list (t_Slice u8) = [data; data] in
       FStar.Pervasives.assert_norm (List.Tot.length l == 2);
-      Rust_primitives.Hax.array_of_list 2 l in
-    EquivImplSpec.Sponge.Arm64.Driver.lemma_keccak2_arm64
-      (mk_usize 144) (mk_u8 6) inputs digest (dummy <: t_Slice u8)
+      Rust_primitives.Hax.array_of_list 2 l
+    in
+    EquivImplSpec.Sponge.Arm64.Driver.lemma_keccak2_arm64 (mk_usize 144)
+      (mk_u8 6)
+      inputs
+      digest
+      (dummy <: t_Slice u8)
   in
   let (tmp0: t_Slice u8), (tmp1: t_Array u8 (mk_usize 28)) =
     Libcrux_sha3.Generic_keccak.Simd128.keccak2 (mk_usize 144)
@@ -45,6 +51,10 @@ let sha224 (digest data: t_Slice u8)
   let _:Prims.unit = () in
   digest
 
+#pop-options
+
+#push-options "--fuel 0 --ifuel 1 --z3rlimit 200 --split_queries always"
+
 /// A SHA3 256 implementation.
 let sha256 (digest data: t_Slice u8)
     : Prims.Pure (t_Slice u8)
@@ -59,17 +69,23 @@ let sha256 (digest data: t_Slice u8)
             bool) /\
           (digest_future <: t_Slice u8) ==
           (Hacspec_sha3.Sponge.keccak (Core_models.Slice.impl__len #u8 digest)
-              (mk_usize 136) (mk_u8 6) data
+              (mk_usize 136)
+              (mk_u8 6)
+              data
             <:
             t_Slice u8)) =
   let dummy:t_Array u8 (mk_usize 32) = Rust_primitives.Hax.repeat (mk_u8 0) (mk_usize 32) in
   let _:Prims.unit =
-    let inputs : t_Array (t_Slice u8) (mk_usize 2) =
-      let l : list (t_Slice u8) = [ data; data ] in
+    let inputs:t_Array (t_Slice u8) (mk_usize 2) =
+      let l:list (t_Slice u8) = [data; data] in
       FStar.Pervasives.assert_norm (List.Tot.length l == 2);
-      Rust_primitives.Hax.array_of_list 2 l in
-    EquivImplSpec.Sponge.Arm64.Driver.lemma_keccak2_arm64
-      (mk_usize 136) (mk_u8 6) inputs digest (dummy <: t_Slice u8)
+      Rust_primitives.Hax.array_of_list 2 l
+    in
+    EquivImplSpec.Sponge.Arm64.Driver.lemma_keccak2_arm64 (mk_usize 136)
+      (mk_u8 6)
+      inputs
+      digest
+      (dummy <: t_Slice u8)
   in
   let (tmp0: t_Slice u8), (tmp1: t_Array u8 (mk_usize 32)) =
     Libcrux_sha3.Generic_keccak.Simd128.keccak2 (mk_usize 136)
@@ -85,6 +101,10 @@ let sha256 (digest data: t_Slice u8)
   let _:Prims.unit = () in
   digest
 
+#pop-options
+
+#push-options "--fuel 0 --ifuel 1 --z3rlimit 200 --split_queries always"
+
 /// A SHA3 384 implementation.
 let sha384 (digest data: t_Slice u8)
     : Prims.Pure (t_Slice u8)
@@ -99,17 +119,23 @@ let sha384 (digest data: t_Slice u8)
             bool) /\
           (digest_future <: t_Slice u8) ==
           (Hacspec_sha3.Sponge.keccak (Core_models.Slice.impl__len #u8 digest)
-              (mk_usize 104) (mk_u8 6) data
+              (mk_usize 104)
+              (mk_u8 6)
+              data
             <:
             t_Slice u8)) =
   let dummy:t_Array u8 (mk_usize 48) = Rust_primitives.Hax.repeat (mk_u8 0) (mk_usize 48) in
   let _:Prims.unit =
-    let inputs : t_Array (t_Slice u8) (mk_usize 2) =
-      let l : list (t_Slice u8) = [ data; data ] in
+    let inputs:t_Array (t_Slice u8) (mk_usize 2) =
+      let l:list (t_Slice u8) = [data; data] in
       FStar.Pervasives.assert_norm (List.Tot.length l == 2);
-      Rust_primitives.Hax.array_of_list 2 l in
-    EquivImplSpec.Sponge.Arm64.Driver.lemma_keccak2_arm64
-      (mk_usize 104) (mk_u8 6) inputs digest (dummy <: t_Slice u8)
+      Rust_primitives.Hax.array_of_list 2 l
+    in
+    EquivImplSpec.Sponge.Arm64.Driver.lemma_keccak2_arm64 (mk_usize 104)
+      (mk_u8 6)
+      inputs
+      digest
+      (dummy <: t_Slice u8)
   in
   let (tmp0: t_Slice u8), (tmp1: t_Array u8 (mk_usize 48)) =
     Libcrux_sha3.Generic_keccak.Simd128.keccak2 (mk_usize 104)
@@ -125,6 +151,10 @@ let sha384 (digest data: t_Slice u8)
   let _:Prims.unit = () in
   digest
 
+#pop-options
+
+#push-options "--fuel 0 --ifuel 1 --z3rlimit 200 --split_queries always"
+
 /// A SHA3 512 implementation.
 let sha512 (digest data: t_Slice u8)
     : Prims.Pure (t_Slice u8)
@@ -139,17 +169,23 @@ let sha512 (digest data: t_Slice u8)
             bool) /\
           (digest_future <: t_Slice u8) ==
           (Hacspec_sha3.Sponge.keccak (Core_models.Slice.impl__len #u8 digest)
-              (mk_usize 72) (mk_u8 6) data
+              (mk_usize 72)
+              (mk_u8 6)
+              data
             <:
             t_Slice u8)) =
   let dummy:t_Array u8 (mk_usize 64) = Rust_primitives.Hax.repeat (mk_u8 0) (mk_usize 64) in
   let _:Prims.unit =
-    let inputs : t_Array (t_Slice u8) (mk_usize 2) =
-      let l : list (t_Slice u8) = [ data; data ] in
+    let inputs:t_Array (t_Slice u8) (mk_usize 2) =
+      let l:list (t_Slice u8) = [data; data] in
       FStar.Pervasives.assert_norm (List.Tot.length l == 2);
-      Rust_primitives.Hax.array_of_list 2 l in
-    EquivImplSpec.Sponge.Arm64.Driver.lemma_keccak2_arm64
-      (mk_usize 72) (mk_u8 6) inputs digest (dummy <: t_Slice u8)
+      Rust_primitives.Hax.array_of_list 2 l
+    in
+    EquivImplSpec.Sponge.Arm64.Driver.lemma_keccak2_arm64 (mk_usize 72)
+      (mk_u8 6)
+      inputs
+      digest
+      (dummy <: t_Slice u8)
   in
   let (tmp0: t_Slice u8), (tmp1: t_Array u8 (mk_usize 64)) =
     Libcrux_sha3.Generic_keccak.Simd128.keccak2 (mk_usize 72)
@@ -165,6 +201,10 @@ let sha512 (digest data: t_Slice u8)
   let _:Prims.unit = () in
   digest
 
+#pop-options
+
+#push-options "--fuel 0 --ifuel 1 --z3rlimit 200 --split_queries always"
+
 /// A SHAKE128 implementation.
 let shake128 (v_LEN: usize) (digest: t_Array u8 v_LEN) (data: t_Slice u8)
     : Prims.Pure (t_Array u8 v_LEN)
@@ -173,17 +213,19 @@ let shake128 (v_LEN: usize) (digest: t_Array u8 v_LEN) (data: t_Slice u8)
         fun digest_future ->
           let digest_future:t_Array u8 v_LEN = digest_future in
           (digest_future <: t_Array u8 v_LEN) ==
-          (Hacspec_sha3.Sponge.keccak v_LEN (mk_usize 168) (mk_u8 31) data
-            <:
-            t_Array u8 v_LEN)) =
+          (Hacspec_sha3.Sponge.keccak v_LEN (mk_usize 168) (mk_u8 31) data <: t_Array u8 v_LEN)) =
   let dummy:t_Array u8 v_LEN = Rust_primitives.Hax.repeat (mk_u8 0) v_LEN in
   let _:Prims.unit =
-    let inputs : t_Array (t_Slice u8) (mk_usize 2) =
-      let l : list (t_Slice u8) = [ data; data ] in
+    let inputs:t_Array (t_Slice u8) (mk_usize 2) =
+      let l:list (t_Slice u8) = [data; data] in
       FStar.Pervasives.assert_norm (List.Tot.length l == 2);
-      Rust_primitives.Hax.array_of_list 2 l in
-    EquivImplSpec.Sponge.Arm64.Driver.lemma_keccak2_arm64
-      (mk_usize 168) (mk_u8 31) inputs (digest <: t_Slice u8) (dummy <: t_Slice u8)
+      Rust_primitives.Hax.array_of_list 2 l
+    in
+    EquivImplSpec.Sponge.Arm64.Driver.lemma_keccak2_arm64 (mk_usize 168)
+      (mk_u8 31)
+      inputs
+      (digest <: t_Slice u8)
+      (dummy <: t_Slice u8)
   in
   let (tmp0: t_Array u8 v_LEN), (tmp1: t_Array u8 v_LEN) =
     Libcrux_sha3.Generic_keccak.Simd128.keccak2 (mk_usize 168)
@@ -199,6 +241,10 @@ let shake128 (v_LEN: usize) (digest: t_Array u8 v_LEN) (data: t_Slice u8)
   let _:Prims.unit = () in
   digest
 
+#pop-options
+
+#push-options "--fuel 0 --ifuel 1 --z3rlimit 200 --split_queries always"
+
 /// A SHAKE256 implementation.
 let shake256 (v_LEN: usize) (digest: t_Array u8 v_LEN) (data: t_Slice u8)
     : Prims.Pure (t_Array u8 v_LEN)
@@ -207,17 +253,19 @@ let shake256 (v_LEN: usize) (digest: t_Array u8 v_LEN) (data: t_Slice u8)
         fun digest_future ->
           let digest_future:t_Array u8 v_LEN = digest_future in
           (digest_future <: t_Array u8 v_LEN) ==
-          (Hacspec_sha3.Sponge.keccak v_LEN (mk_usize 136) (mk_u8 31) data
-            <:
-            t_Array u8 v_LEN)) =
+          (Hacspec_sha3.Sponge.keccak v_LEN (mk_usize 136) (mk_u8 31) data <: t_Array u8 v_LEN)) =
   let dummy:t_Array u8 v_LEN = Rust_primitives.Hax.repeat (mk_u8 0) v_LEN in
   let _:Prims.unit =
-    let inputs : t_Array (t_Slice u8) (mk_usize 2) =
-      let l : list (t_Slice u8) = [ data; data ] in
+    let inputs:t_Array (t_Slice u8) (mk_usize 2) =
+      let l:list (t_Slice u8) = [data; data] in
       FStar.Pervasives.assert_norm (List.Tot.length l == 2);
-      Rust_primitives.Hax.array_of_list 2 l in
-    EquivImplSpec.Sponge.Arm64.Driver.lemma_keccak2_arm64
-      (mk_usize 136) (mk_u8 31) inputs (digest <: t_Slice u8) (dummy <: t_Slice u8)
+      Rust_primitives.Hax.array_of_list 2 l
+    in
+    EquivImplSpec.Sponge.Arm64.Driver.lemma_keccak2_arm64 (mk_usize 136)
+      (mk_u8 31)
+      inputs
+      (digest <: t_Slice u8)
+      (dummy <: t_Slice u8)
   in
   let (tmp0: t_Array u8 v_LEN), (tmp1: t_Array u8 v_LEN) =
     Libcrux_sha3.Generic_keccak.Simd128.keccak2 (mk_usize 136)
